Experiment with a natural number index that records recursion level.

src/Language/PlutusIR/Semantics/SemanticEquivalence/Def.v
@@ -4,200 +4,161 @@ Require Import PlutusCert.Language.PlutusIR.Semantics.Static.
 Require Import PlutusCert.Language.PlutusIR.Semantics.Static.Implementations.Named.
 Require Import PlutusCert.Language.PlutusIR.Semantics.Dynamic.
 
-Notation beta_reduce := (beta_reduce tyname binderTyname substituteT).
+Notation beta_reduce := (beta_reduce).
+
+Definition terminates := fun t => exists v, t ==> v.
 
 (* Note: The cases for Ty_Forall and and Ty_IFix make use of
    type substitution and beta reduction. However, Coq can then not
    guess the decreasing argument of fix anymore. *)
-Fixpoint R (T : Ty) (ctx_K : partial_map Kind) (t1 t2 : Term) : Prop :=
-  (empty, ctx_K) |-+ t1 : T /\
-  (empty, ctx_K) |-+ t2 : T /\
-  exists v1 v2,
-    t1 ==> v1 /\
-    t2 ==> v2 /\
-    match T with
-    | Ty_Forall X K T0 => 
-        forall t0_1 t0_2,
-          v1 = TyAbs X K t0_1 ->
-          v2 = TyAbs X K t0_2 ->
-          R T0 (X |-> K ; ctx_K) t0_1 t0_2
-    | Ty_Fun T1 T2 => 
-        forall s1 s2,
-          R T1 ctx_K s1 s2 ->
-          R T2 ctx_K (Apply v1 s1) (Apply v2 s2)
-    | Ty_Builtin st => 
-        v1 = v2
-    | Ty_IFix F T0 => 
-        (*
-        forall X K,
-          empty |-* T : K ->
-          R (beta_reduce (unwrapIFix F X K T0)) (Unwrap v1) (Unwrap v2)
-        *)
-        True
-    |_ => False
-    end.
+Fixpoint R (k : nat) (T : Ty) (t1 t2 : Term) {struct k} : Prop :=
+  emptyContext |-+ t1 : T /\
+  emptyContext |-+ t2 : T /\
+  forall v1,
+    t1 ==> v1 ->
+    exists v2,
+      t2 ==> v2 /\
+        match T with
+        | Ty_Forall X K T0 => 
+            match k with 
+            | 0 => 
+                False
+            | S k' =>
+                forall t0_1 t0_2 T',
+                  v1 = TyAbs X K t0_1 ->
+                  v2 = TyAbs X K t0_2 ->
+                  forall H : emptyContext |-* T' : K,
+                  R k' (beta_reduce (substituteT X T' T0)) (TyInst v1 T') (TyInst v2 T')
+            end
+        | Ty_Fun T1 T2 => 
+            match k with
+            | 0 =>
+                False
+            | S k' =>
+                forall s1 s2,
+                  R k' T1 s1 s2 ->
+                  R k' T2 (Apply v1 s1) (Apply v2 s2)
+            end
+        | Ty_Builtin st => 
+            v1 = v2
+        | Ty_IFix F T0 => 
+            match k with
+            | 0 =>
+                False
+            | S k' =>
+                forall X K,
+                  emptyContext |-* T : K ->
+                  R k' (beta_reduce (unwrapIFix F X K T0)) (Unwrap v1) (Unwrap v2)
+            end
+        |_ => False
+        end.
 
-Lemma R_typable_emptyT : forall T ctxK t1 t2,
-    R T ctxK t1 t2 ->
-    (empty, ctxK) |-+ t1 : T /\ (empty, ctxK) |-+ t2 : T.
-Proof. intros. destruct T; destruct H as [Ht1 [Ht2 _]]; auto. Qed.
+Lemma R_typable_empty : forall k T t1 t2,
+    R k T t1 t2 ->
+    emptyContext |-+ t1 : T /\ emptyContext |-+ t2 : T.
+Proof. intros. destruct k, T; destruct H as [Ht1 [Ht2 _]]; auto. Qed.
 
-Lemma R_typable_emptyT_1 : forall T ctxK t1 t2,
-    R T ctxK t1 t2 ->
-    (empty, ctxK) |-+ t1 : T.
-Proof. intros. destruct (R_typable_emptyT _ _ _ _ H). assumption. Qed.
+Lemma R_typable_empty_1 : forall k T t1 t2,
+    R k T t1 t2 ->
+    emptyContext |-+ t1 : T.
+Proof. intros. destruct (R_typable_empty _ _ _ _ H). assumption. Qed.
 
-Lemma R_typable_emptyT_2 : forall T ctxK t1 t2,
-    R T ctxK t1 t2 ->
-    (empty, ctxK) |-+ t2 : T.
-Proof. intros. destruct (R_typable_emptyT _ _ _ _ H). assumption. Qed.
+Lemma R_typable_empty_2 : forall k T t1 t2,
+    R k T t1 t2 ->
+    emptyContext |-+ t2 : T.
+Proof. intros. destruct (R_typable_empty _ _ _ _ H). assumption. Qed.
 
-Lemma R_evaluable : forall T ctxK t1 t2,
-    R T ctxK t1 t2 ->
+Lemma R_evaluable : forall k T t1 t2,
+    terminates t1 ->
+    R k T t1 t2 ->
     exists v1 v2, t1 ==> v1 /\ t2 ==> v2.
-Proof. intros. destruct T; destruct H as [_ [_ [v1 [v2 [Hev1 [Hev2 _]]]]]]; eauto. Qed.
+Proof. intros. destruct H. destruct k, T; destruct H0 as [_ [_ [v1 [Hev2 _]]]]; eauto. Qed.
 
-Lemma R_evaluable_1 : forall T ctxK t1 t2,
-    R T ctxK t1 t2 ->
+Lemma R_evaluable_1 : forall k T t1 t2,
+    terminates t1 ->
+    R k T t1 t2 ->
     exists v1, t1 ==> v1.
-Proof. intros. destruct (R_evaluable _ _ _ _ H) as [v1 [_ [Hev1 _]]]. eauto. Qed.
+Proof. intros. destruct (R_evaluable _ _ _ _ H H0) as [v1 [_ [Hev1 _]]]. eauto. Qed.
 
-Lemma R_evaluable_2 : forall T ctxK t1 t2,
-    R ctxK T t1 t2 ->
+Lemma R_evaluable_2 : forall k T t1 t2,
+    terminates t1 ->
+    R k T t1 t2 ->
     exists v2, t2 ==> v2.
-Proof. intros. destruct (R_evaluable _ _ _ _ H) as [_ [v2 [_ Hev2]]]. eauto. Qed.
+Proof. intros. destruct (R_evaluable _ _ _ _ H H0) as [_ [v2 [_ Hev2]]]. eauto. Qed.
 
-Lemma R_syntactic_equality : forall st ctxK t1 t2,
-    R (Ty_Builtin st) ctxK t1 t2 ->
+Lemma R_syntactic_equality : forall k st t1 t2,
+    terminates t1 ->
+    R k (Ty_Builtin st) t1 t2 ->
     exists v1 v2,
       t1 ==> v1 /\
       t2 ==> v2 /\
       v1 = v2.
-Proof. intros. destruct H as [_ [_ [v1 [v2 [Hev1 [Hev2 Heq]]]]]]. eauto. Qed.
+Proof. intros. destruct H. destruct k; destruct H0 as [_ [_ [v2 [Hev2 Heq]]]]; eauto. Qed.
 
-Lemma R_functional_extensionality : forall T1 T2 ctxK t1 t2,
-  R (Ty_Fun T1 T2) ctxK t1 t2 ->
-  exists v1 v2,
-    t1 ==> v1 /\
-    t2 ==> v2 /\
-    (forall s1 s2,
-      R T1 ctxK s1 s2 ->
-      R T2 ctxK (Apply v1 s1) (Apply v2 s2)).
-Proof. intros. destruct H as [_ [_ [v1 [v2 [Hev1 [Hev2 Hfe]]]]]]. eauto. Qed.
-
-Lemma R_falsity : forall ctxK t1 t2,
-  (forall a, ~(R (Ty_Var a) ctxK t1 t2)) /\
-  (forall bX K T, ~(R (Ty_Lam bX K T) ctxK t1 t2)) /\
-  (forall T1 T2, ~(R (Ty_App T1 T2) ctxK t1 t2)).
-Proof. 
-  split.
-  - intros. intro Hcon. destruct Hcon as [_ [_ [_ [_ [_ [_ Hfalse]]]]]]. destruct Hfalse.
-  - split.
-    + intros. intro Hcon. edestruct Hcon as [_ [_ [_ [_ [_ [_ Hfalse]]]]]]. destruct Hfalse.
-    + intros. intro Hcon. edestruct Hcon as [_ [_ [_ [_ [_ [_ Hfalse]]]]]]. destruct Hfalse.
-Qed.
-
-(* TODO: Possible fixes for R require a proof of well-founded recursion. I've tried out some things
-   below, but I have not founda solution yet. *)
-(* https://coq.inria.fr/refman/addendum/program.html *)
-(* http://adam.chlipala.net/cpdt/html/Cpdt.GeneralRec.html *)
-
-Fixpoint countBindingLocations (T : Ty) : nat := 
-  match T with
-  | Ty_Var X => 0
-  | Ty_Fun T1 T2 => countBindingLocations T1 + countBindingLocations T2
-  | Ty_IFix F T0 => countBindingLocations F + countBindingLocations T0
-  | Ty_Forall X K T0 => 1 + countBindingLocations T0
-  | Ty_Builtin st => 0
-  | Ty_Lam X K T0 => 1 + countBindingLocations T0       
-  | Ty_App T1 T2 => countBindingLocations T1 + countBindingLocations T2  
-  end.
-
-Program Fixpoint R'' (T : Ty) (t1 t2 : Term) {measure (countBindingLocations T)} : Prop :=
-  emptyContext |-+ t1 : T /\
-  emptyContext |-+ t2 : T /\
-  exists v1 v2,
-    t1 ==> v1 /\
-    t2 ==> v2 /\
-    match T with
-    | Ty_Forall X K T0 => 
-        forall t0 T',
-          v1 = TyAbs X K t0 ->
-          v2 = TyAbs X K t0 ->
-          emptyContext |-* T' : K ->
-          R'' (Named.beta_reduce (substituteT X T' T0)) (TyInst v1 T') (TyInst v2 T')
-    | Ty_Fun T1 T2 => 
-        forall s1 s2,
-          R'' T1 s1 s2 ->
-          R'' T2 (Apply v1 s1) (Apply v2 s2)
-    | Ty_Builtin st => 
-        v1 = v2
-    | Ty_IFix F T0 => 
-        forall X K,
-          emptyContext |-* T : K ->
-          R'' (Named.beta_reduce (unwrapIFix F X K T0)) (Unwrap v1) (Unwrap v2)
-    |_ => False
-    end.
-Next Obligation. Admitted.
-Next Obligation. Admitted.
-Next Obligation. Admitted.
-Next Obligation. Admitted.
-Next Obligation. Admitted.
-Next Obligation. Admitted.
-Next Obligation. Admitted.
-Next Obligation. Admitted.
-
-(* WF by countBindingLocations and size? *)
-Equations R' (T : Ty) (t1 t2 : Term) : Prop by wf (countBindingLocations T) :=
-  R' T t1 t2 =>
-    emptyContext |-+ t1 : T /\
-    emptyContext |-+ t2 : T /\
+Lemma R_functional_extensionality : forall k' T1 T2 t1 t2,
+    terminates t1 ->
+    R (S k') (Ty_Fun T1 T2) t1 t2 ->
     exists v1 v2,
       t1 ==> v1 /\
       t2 ==> v2 /\
-      match T with
-      | Ty_Forall X K T0 => 
-          forall t0 T',
-            v1 = TyAbs X K t0 ->
-            v2 = TyAbs X K t0 ->
-            emptyContext |-* T' : K ->
-            R' (Named.beta_reduce (substituteT X T' T0)) (TyInst v1 T') (TyInst v2 T')
-      | Ty_Fun T1 T2 => 
-          forall s1 s2,
-            R' T1 s1 s2 ->
-            R' T2 (Apply v1 s1) (Apply v2 s2)
-      | Ty_Builtin st => 
-          v1 = v2
-      | Ty_IFix F T0 => 
-          forall X K,
-            emptyContext |-* T : K ->
-            R' (Named.beta_reduce (unwrapIFix F X K T0)) (Unwrap v1) (Unwrap v2)
-      |_ => False
-      end.
-      
-
-Fail Inductive R : Ty -> Term -> Term -> Prop :=
-  | R_ : forall t1 t2 T,
-      (emptyContext |-+ t1 : T /\
-      emptyContext |-+ t2 : T /\
-      exists v1 v2,
-        t1 ==> v1 /\
-        t2 ==> v2 /\
-        R2 T v1 v2) ->
-      R T t1 t2
-      
-with R2 : Ty -> Term -> Term -> Prop :=
-  | R2_TyForall : forall X K T0,
-      forall v1 v2 t0 T' S,
-        v1 = TyAbs X K t0 ->
-        v2 = TyAbs X K t0 ->
-        emptyContext |-+ t0 : T0 ->
-        emptyContext |-* T' : K ->
-        substituteT X T' T0 =b S ->
-        R S (TyInst v1 T') (TyInst v2 T') ->
-        R2 (Ty_Forall X K T0) v1 v2
-  | R2_TyFun : forall T1 T2 v1 v2,
       (forall s1 s2,
-        R T1 s1 s2 ->
-        R T2 (Apply v1 s1) (Apply v2 s2)) ->
-      R2 (Ty_Fun T1 T2) v1 v2.
+        R k' T1 s1 s2 ->
+        R k' T2 (Apply v1 s1) (Apply v2 s2)).
+Proof. intros. destruct H. destruct H0 as [_ [_ [v2 [Hev2 Hfe]]]]; eauto. Qed.
+
+Lemma R_impossible_type : forall k t1 t2,
+    terminates t1 ->
+    (forall a, ~(R k (Ty_Var a) t1 t2)) /\
+    (forall bX K T, ~(R k (Ty_Lam bX K T) t1 t2)) /\
+    (forall T1 T2, ~(R k (Ty_App T1 T2) t1 t2)).
+Proof.
+  intros. destruct H. 
+  split; try split; try solve [intros; intro Hcon; destruct k; destruct Hcon as [_ [_ [_ [_ Hfalse]]]]; eauto].
+Qed.
+
+Lemma R_impossible_k : forall t1 t2,
+    terminates t1 ->
+    (forall T1 T2, ~(R 0 (Ty_Fun T1 T2) t1 t2)) /\
+    (forall X K T0, ~(R 0 (Ty_Forall X K T0) t1 t2)).
+Proof.
+  intros. destruct H.
+  split; intros; try solve [intros Hcon; destruct Hcon as [_ [_ [_ [_ Hfls]]]]; eauto].
+Qed.
+
+Lemma R_nontermination : forall k T t1 t2,
+    ~(terminates t1) ->
+    emptyContext |-+ t1 : T ->
+    emptyContext |-+ t2 : T ->
+    R k T t1 t2.
+Proof. intros. destruct k; destruct T; try solve [split; eauto; split; eauto; intros v1 Hcon; exfalso; apply H; exists v1; auto]. Qed.
+
+Axiom skip: forall P, P.
+
+Lemma R_monotone : forall k1 k2 T t1 t2,
+  terminates t1 ->
+  R k1 T t1 t2 ->
+  k1 < k2 ->
+  R k2 T t1 t2.
+Proof.
+  intros k1 k2 T.
+  generalize dependent k2.
+  generalize dependent k1.
+  induction T; intros.
+  - apply R_impossible_type in H0; eauto. destruct H0.
+  - destruct k1; destruct k2.
+    + apply PeanoNat.Nat.nlt_0_r in H1. destruct H1.
+    + apply R_impossible_k in H0. destruct H0. assumption.
+    + apply PeanoNat.Nat.nlt_0_r in H1. destruct H1.
+    + destruct (R_typable_empty _ _ _ _ H0).
+      split; auto.
+      split; auto.
+      destruct (R_functional_extensionality _ _ _ _ _ H H0) as [v1 [v2 [Hev1 [Hev2 Hfe]]]].
+      intros.
+      exists v2.
+      split; auto.
+      assert (v0 = v1) by (eapply eval__deterministic; eauto).
+      subst.
+      intros.
+      apply skip.
+  - destruct k1; destruct k2; destruct (R_typable_empty _ _ _ _ H0); eauto.
+Abort.
