src/Language/PlutusIR/Semantics/SemanticEquivalence/ReductionInvariance.v
@@ -1,0 +1,73 @@
+Require Import PlutusCert.Language.PlutusIR.
+Import NamedTerm.
+Require Import PlutusCert.Language.PlutusIR.Semantics.Static.
+Require Import PlutusCert.Language.PlutusIR.Semantics.Static.Implementations.Named.
+Require Import PlutusCert.Language.PlutusIR.Semantics.Dynamic.
+Require Import PlutusCert.Language.PlutusIR.Semantics.SemanticEquivalence.Def.
+
+Lemma eval_preserves_termination : forall t v,
+    terminates t ->
+    t ==> v ->
+    terminates v.
+Proof. intros. exists v. apply eval_value. eapply eval_to_value. apply H0. Qed.
+
+Lemma eval_preserves_R_left : forall k T t1 v1 t2,
+    terminates t1 ->
+    t1 ==> v1 ->
+    R k T t1 t2 ->
+    R k T v1 t2.
+Proof. Abort.
+
+Lemma eval_preserves_R_right : forall k T t1 t2 v2,
+    terminates t1 ->
+    t2 ==> v2 ->
+    R k T t1 t2 ->
+    R k T t1 v2.
+Proof. Abort.
+
+Lemma eval_preserves_R : forall k T t1 v1 t2 v2,
+    terminates t1 ->
+    t1 ==> v1 ->
+    t2 ==> v2 ->
+    R k T t1 t2 ->
+    R k T v1 v2.
+Proof.
+  intros k T t1 v1 t2 v2 Hterm1 Hev1 Hev2 R.
+  (*
+  apply eval_preserves_R_left with t1; auto.
+  apply eval_preserves_R_right with t2; auto.
+  *)
+Abort.
+
+Lemma eval_preserved_R_left : forall k T t1 v1 t2,
+    emptyContext |-+ t1 : T ->
+    terminates t1 ->
+    t1 ==> v1 ->
+    R k T v1 t2 ->
+    R k T t1 t2.
+Proof. Abort.
+
+Lemma eval_preserved_R_right : forall k T t1 t2 v2,
+    emptyContext |-+ t2 : T ->
+    terminates t1 ->
+    t2 ==> v2 ->
+    R k T t1 v2 ->
+    R k T t1 t2.
+Proof. Abort.
+
+Lemma eval_preserved_R : forall k T t1 t2 v1 v2,
+    emptyContext |-+ t1 : T ->
+    emptyContext |-+ t2 : T ->
+    terminates t1 ->
+    t1 ==> v1 ->
+    t2 ==> v2 ->
+    R k T v1 v2 ->
+    R k T t1 t2.
+Proof.
+  intros k T t1 t2 v1 v2 Htyp_t1 Htyp_t2 Hterm1 Hev1 Hev2 R.
+  (*
+  apply eval_preserved_R_left with v1; auto.
+  apply eval_preserved_R_right with v2; auto.
+  apply eval_preserves_termination with t1; auto.
+  *)
+Abort.
