src/Language/PlutusIR/Semantics/TypeSafety/Progress.v
@@ -170,3 +170,5 @@ Proof.
            ++ apply H10.
            ++ apply H11.
 Abort.
+
+End e.
